ulib/FStar.BufferNG.fst
@@ -1,6 +1,5 @@
 module FStar.BufferNG
 module HH = FStar.HyperStack
-module DM = FStar.DependentMap
 module HS = FStar.HyperStack
 module HST = FStar.HyperStack.ST
 module P = FStar.Pointer
